Add partial version with equality_modulo for heaps

vale/code/arch/x64/X64.Vale.Lemmas.fst
@@ -2,6 +2,7 @@ module X64.Vale.Lemmas
 open X64.Machine_s
 open X64.Vale.State
 open X64.Vale.StateLemmas
+open X64.Vale.StateEqSemantics
 module BS = X64.Bytes_Semantics_s
 module TS = X64.Taint_Semantics_s
 module ME = X64.Memory_s
@@ -9,7 +10,158 @@ module ME = X64.Memory_s
 friend X64.Memory
 friend X64.Vale.StateLemmas
 
-#reset-options "--initial_fuel 2 --max_fuel 2 --z3rlimit 20"
+#reset-options "--initial_fuel 2 --max_fuel 2 --max_ifuel 2 --initial_ifuel 2 --z3rlimit 20"
+(*
+
+(*
+val eval_operand_eq_all (o:operand) (s1 s2:BS.state) : Lemma
+  (requires state_eq_BS s1 s2)
+  (ensures BS.eval_operand o s1 == BS.eval_operand o s2) 
+  [SMTPat (BS.eval_operand o s1); SMTPat (state_eq_BS s1 s2)]
+
+let eval_operand_eq_all o s1 s2 = ()
+
+val eq_all_havoc (ins:BS.ins) (s1 s2:BS.state) : Lemma
+  (requires state_eq_BS s1 s2)
+  (ensures BS.havoc s1 ins == BS.havoc s2 ins)
+  [SMTPat (BS.havoc s1 ins); SMTPat (state_eq_BS s1 s2)]
+
+let eq_all_havoc ins s1 s2 = admit()
+
+val update_operand_preserve_flags_eq_all (o:operand) (v:nat64) (s1 s2:BS.state) : Lemma
+  (requires state_eq_BS s1 s2)
+  (ensures state_eq_BS
+    (BS.update_operand_preserve_flags' o v s1)
+    (BS.update_operand_preserve_flags' o v s2)
+  )
+  [SMTPat (BS.update_operand_preserve_flags' o v s1); SMTPat (state_eq_BS s1 s2)]
+
+let update_operand_preserve_flags_eq_all o v s1 s2 = match o with
+  | OMem m -> ()
+  | OReg r -> 
+    let s1' = BS.update_operand_preserve_flags' o v s1 in
+    let s2' = BS.update_operand_preserve_flags' o v s2 in
+    assert (FunctionalExtensionality.feq s1'.BS.regs s2'.BS.regs)
+  | _ -> ()
+
+val update_operand_eq_all (o:operand) (ins:BS.ins) (v:nat64) (s1 s2:BS.state) : Lemma
+  (requires state_eq_BS s1 s2)
+  (ensures state_eq_BS
+    (BS.update_operand' o ins v s1)
+    (BS.update_operand' o ins v s2)
+  )
+  [SMTPat (BS.update_operand' o ins v s1); SMTPat (state_eq_BS s1 s2)]
+
+let update_operand o ins v s1 s2 = ()
+*)
+val eval_ins_bs_eq_all (c:BS.ins) (s1 s2:BS.state) : Lemma
+  (requires state_eq_BS s1 s2)
+  (ensures state_eq_BS (BS.run (BS.eval_ins c) s1) (BS.run (BS.eval_ins c) s2))
+
+let eval_ins_bs_eq_all c s1 s2 = admit() (*
+  if BS.Add64? c then (
+    let BS.Add64 dst src = c in
+    let s1' = BS.run (BS.check (BS.valid_operand src)) s1 in
+    let s2' = BS.run (BS.check (BS.valid_operand src)) s2 in
+    let s1' = BS.run (BS.check (BS.valid_dst_operand dst)) s1' in
+    let s2' = BS.run (BS.check (BS.valid_dst_operand dst)) s2' in
+    assert (state_eq_BS s1' s2');
+    ()
+  ) else admit()
+*)
+(*
+val eq_update_taint_list 
+  (memTaint1 memTaint2:memTaint_t)
+  (dsts:list operand)
+  (t:taint)
+  (s1 s2:BS.state) : Lemma
+  (requires memTaint1 == memTaint2 /\ state_eq_BS s1 s2)
+  (ensures TS.update_taint_list memTaint1 dsts t s1 == TS.update_taint_list memTaint2 dsts t s2)
+  (decreases %[dsts])
+
+let rec eq_update_taint_list memTaint1 memTaint2 dsts t s1 s2 = match dsts with
+  | [] -> ()
+  | a :: q -> eq_update_taint_list
+    (TS.update_taint memTaint1 a t s1)
+    (TS.update_taint memTaint2 a t s2)
+    q t s1 s2
+
+val eq_all_taint_match_list: 
+  (srcs:list operand) ->
+  (t:taint) ->
+  (memTaint1:memTaint_t) ->
+  (memTaint2:memTaint_t) ->
+  (s1:BS.state) ->
+  (s2:BS.state) ->
+  Lemma 
+    (requires memTaint1 == memTaint2 /\ state_eq_BS s1 s2)
+    (ensures TS.taint_match_list srcs t memTaint1 s1 == TS.taint_match_list srcs t memTaint2 s2)
+
+let rec eq_all_taint_match_list srcs t memTaint1 memTaint2 s1 s2 =
+  match srcs with
+  | [] -> ()
+  | a::q -> eq_all_taint_match_list q t memTaint1 memTaint2 s1 s2
+
+val eval_ins_same_memTaint (c:TS.tainted_ins) (s1 s2:TS.traceState) : Lemma
+  (requires state_eq_S s1 s2)
+  (ensures (TS.taint_eval_ins c s1).TS.memTaint == (TS.taint_eval_ins c s2).TS.memTaint)
+
+let eval_ins_same_memTaint c s1 s2 =
+  let i, dsts, srcs = c.TS.ops in
+  let t = c.TS.t in
+  if BS.Mulx64? i then (
+    let s1' = BS.run (BS.check (TS.taint_match_list srcs t s1.TS.memTaint)) s1.TS.state in
+    let s2' = BS.run (BS.check (TS.taint_match_list srcs t s2.TS.memTaint)) s2.TS.state in  
+    let BS.Mulx64 dst_hi dst_lo src = i in
+    eq_all_taint_match_list srcs t s1.TS.memTaint s2.TS.memTaint s1.TS.state s2.TS.state;
+    let lo1 = FStar.UInt.mul_mod #64 (BS.eval_reg Rdx s1') (BS.eval_operand src s1') in
+    let lo2 = FStar.UInt.mul_mod #64 (BS.eval_reg Rdx s2') (BS.eval_operand src s2') in
+    let s1'' = BS.update_operand_preserve_flags' dst_lo lo1 s1' in
+    let s2'' = BS.update_operand_preserve_flags' dst_lo lo2 s2' in
+    let memTaint1 = TS.update_taint s1.TS.memTaint dst_lo t s1' in
+    let memTaint2 = TS.update_taint s2.TS.memTaint dst_lo t s2' in
+    let memTaint1 = TS.update_taint memTaint1 dst_hi t s1'' in
+    let memTaint2 = TS.update_taint memTaint2 dst_hi t s2'' in
+    assert (memTaint1 == memTaint2)
+  )
+  else if BS.MOVDQU? i then ()
+  else if BS.Push? i then ()
+  else if BS.Mulx64? i then ()
+  else 
+    let s1' = BS.run (BS.check (TS.taint_match_list srcs t s1.TS.memTaint)) s1.TS.state in
+    let s2' = BS.run (BS.check (TS.taint_match_list srcs t s2.TS.memTaint)) s2.TS.state in
+    eq_all_taint_match_list srcs t s1.TS.memTaint s2.TS.memTaint s1.TS.state s2.TS.state;
+    eq_update_taint_list s1.TS.memTaint s2.TS.memTaint dsts t s1' s2'
+*)
+
+val eval_ins_eq_all (c:TS.tainted_ins) : Lemma
+  (ensures (forall (s1 s2:TS.traceState).{:pattern (TS.taint_eval_ins c s1); (TS.taint_eval_ins c s2)}
+    state_eq_S s1 s2 ==>
+    state_eq_S (TS.taint_eval_ins c s1) (TS.taint_eval_ins c s2)
+  ))
+
+let eval_ins_eq_all c = admit() (*
+  let i, dsts, srcs = c.TS.ops in
+  let t = c.TS.t in
+  let aux (s1 s2:TS.traceState) : Lemma 
+    (requires state_eq_S s1 s2)
+    (ensures state_eq_S (TS.taint_eval_ins c s1) (TS.taint_eval_ins c s2)) = 
+    eval_ins_same_memTaint c s1 s2;
+    if BS.MOVDQU? i then (
+      let BS.MOVDQU dst src = i in
+      let s1' = BS.run (BS.check (TS.taint_match128 src t s1.TS.memTaint)) s1.TS.state in
+      let s2' = BS.run (BS.check (TS.taint_match128 src t s2.TS.memTaint)) s2.TS.state in
+      eval_ins_bs_eq_all i s1' s2'
+    ) else (
+      let s1' = BS.run (BS.check (TS.taint_match_list srcs t s1.TS.memTaint)) s1.TS.state in
+      let s2' = BS.run (BS.check (TS.taint_match_list srcs t s2.TS.memTaint)) s2.TS.state in
+      eq_all_taint_match_list srcs t s1.TS.memTaint s2.TS.memTaint s1.TS.state s2.TS.state;
+      eval_ins_bs_eq_all i s1' s2'
+    )
+  in
+  Classical.forall_intro_2 (fun s1 s2 -> Classical.move_requires (fun () -> aux s1 s2) ())
+*)
+*)
 
 val eval_code_eq_all (c:code) (f:fuel) : Lemma
   (ensures (forall (s1 s2:TS.traceState).{:pattern (TS.taint_eval_code c f s1); (TS.taint_eval_code c f s2)}
@@ -32,9 +184,11 @@ val eval_while_eq_all (c:code) (f:fuel) : Lemma
   ))
   (decreases %[f; c; 0])
 
+#set-options "--z3rlimit 50"
+
 let rec eval_code_eq_all c f =
   match c with
-  | Ins ins -> ()
+  | Ins ins -> eval_ins_eq_all ins
   | Block cs -> eval_codes_eq_all cs f
   | IfElse _ ct cf -> eval_code_eq_all ct f; eval_code_eq_all cf f
   | While _ _ -> eval_while_eq_all c f
