vale/code/arch/x64/X64.Vale.StateEqSemantics.fsti
@@ -1,0 +1,10 @@
+module X64.Vale.StateEqSemantics
+
+open X64.Vale.StateLemmas
+module TS = X64.Taint_Semantics_s
+
+val eval_ins_eq_all (c:TS.tainted_ins) : Lemma
+  (ensures (forall (s1 s2:TS.traceState).{:pattern (TS.taint_eval_ins c s1); (TS.taint_eval_ins c s2)}
+    state_eq_S s1 s2 ==>
+    state_eq_S (TS.taint_eval_ins c s1) (TS.taint_eval_ins c s2)
+  ))
